Implement JSON decoding for most Bril constructs

bril-coq/theories/Instruction.v
@@ -1,36 +1,264 @@
-Require Import Coq.Strings.String.
+From Coq Require Import Strings.String.
+From ExtLib Require Import Monad.
+From JSON Require Import JSON Decode Encode.
+Require Import Util.JSON.
+Require Literal Typ.
 
-Require Literal.
+Module Dest.
+
+  (** Represents the destination of a Bril instruction *)
+  Record t := {
+    name : string;
+    typ : Typ.t;
+  }.
+
+  Global Instance JDecode_Dest : JDecode t :=
+    fun j =>
+      name <- (get_string =<< member "dest" j) ;;
+      typ <- (decode =<< member "type" j) ;;
+      ret {| name := name; typ := typ |}.
+
+End Dest.
+
+(* Newtypes to prevent confusion between destinations and operands *)
+
+(** Represents an argument to a Bril instruction *)
+Variant operand := Op (op : string).
+
+Global Instance JDecode_Operand : JDecode operand :=
+  fun j => Op <$> get_string j.
+
+(** Represents a Bril label *)
+Variant label := Label (label : string).
+
+Global Instance JDecode_Label : JDecode label :=
+  fun j => Label <$> get_string j.
+
+(** Represents the name of a Bril function *)
+Variant function := Func (func : string).
+
+Global Instance JDecode_Func : JDecode function :=
+  fun j => Func <$> get_string j.
+
+Definition decode_pair {T} `{JDecode T} : JDecode (T * T) :=
+  fun j =>
+    lst <- @decode (list T) decode__list j ;;
+    match lst with
+    | [x; y] => ret (x, y)
+    | _ => inl "List does not have two elements"
+    end.
 
 (** Represents a Bril instruction *)
 Variant t :=
 
   (* Arithmetic *)
-  | Add (dest : string) (x : string) (y : string)
-  | Mul (dest : string) (x : string) (y : string)
-  | Sub (dest : string) (x : string) (y : string)
-  | Div (dest : string) (x : string) (y : string)
+  | Add (dest : Dest.t) (x : operand) (y : operand)
+  | Mul (dest : Dest.t) (x : operand) (y : operand)
+  | Sub (dest : Dest.t) (x : operand) (y : operand)
+  | Div (dest : Dest.t) (x : operand) (y : operand)
 
   (* Comparison *)
-  | Eq (dest : string) (x : string) (y : string)
-  | Lt (dest : string) (x : string) (y : string)
-  | Gt (dest : string) (x : string) (y : string)
-  | Le (dest : string) (x : string) (y : string)
-  | Ge (dest : string) (x : string) (y : string)
+  | Eq (dest : Dest.t) (x : operand) (y : operand)
+  | Lt (dest : Dest.t) (x : operand) (y : operand)
+  | Gt (dest : Dest.t) (x : operand) (y : operand)
+  | Le (dest : Dest.t) (x : operand) (y : operand)
+  | Ge (dest : Dest.t) (x : operand) (y : operand)
 
   (* Logic *)
-  | Not (dest : string) (x : string)
-  | And (dest : string) (x : string) (y : string)
-  | Or (dest : string) (x : string) (y : string)
+  | Not (dest : Dest.t) (x : operand)
+  | And (dest : Dest.t) (x : operand) (y : operand)
+  | Or (dest : Dest.t) (x : operand) (y : operand)
 
   (* Control *)
-  | Jmp (l : string)
-  | Br (cond : string) (t : string) (f : string)
-  | Call (dest : option string) (name : string) (args : list string)
-  | Ret
+  | Jmp (l : label)
+  | Br (cond : operand) (t : label) (f : label)
+  | Call (dest : option Dest.t) (func : function) (args : list operand)
+  | Ret (val : option operand)
 
   (* Misc *)
-  | Const (dest : string) (lit : Literal.t)
-  | Id (dest : string) (x : string)
-  | Print (args : list string)
+  | Const (dest : Dest.t) (lit : Literal.t)
+  | Id (dest : Dest.t) (x : operand)
+  | Print (args : list operand)
   | Nop.
+
+(** Extract the opcode from an instruction *)
+Definition opcode (instr : Instruction.t) : string :=
+  match instr with
+  | Add _ _ _ => "add"
+  | Mul _ _ _ => "mul"
+  | Sub _ _ _ => "sub"
+  | Div _ _ _ => "div"
+  | Eq _ _ _ => "eq"
+  | Lt _ _ _ => "lt"
+  | Gt _ _ _ => "gt"
+  | Le _ _ _ => "le"
+  | Ge _ _ _ => "ge"
+  | Not _ _ => "not"
+  | And _ _ _ => "and"
+  | Or _ _ _ => "or"
+  | Const _ _ => "const"
+  | Id _ _ => "id"
+  | Call _ _ _ => "call"
+  | Jmp _ => "jmp"
+  | Br _ _ _ => "br"
+  | Ret _ => "ret"
+  | Print _ => "print"
+  | Nop => "nop"
+  end.
+
+(** Extract the destination of an instruction *)
+Definition dest (instr : t) : option Dest.t :=
+  match instr with
+  | Add dst _ _
+  | Mul dst _ _
+  | Sub dst _ _
+  | Div dst _ _
+  | Eq dst _ _
+  | Lt dst _ _
+  | Gt dst _ _
+  | Le dst _ _
+  | Ge dst _ _
+  | Not dst _
+  | And dst _ _
+  | Or dst _ _
+  | Const dst _
+  | Id dst _ => Some dst
+  | Call dst _ _ => dst
+  | Jmp _ | Br _ _ _ | Ret _ | Print _ | Nop => None
+  end.
+
+(** Extract the arguments to an instruction *)
+Definition args (instr : t) : list operand :=
+  match instr with
+  | Add _ x y
+  | Mul _ x y
+  | Sub _ x y
+  | Div _ x y
+  | Eq _ x y
+  | Lt _ x y
+  | Gt _ x y
+  | Le _ x y
+  | Ge _ x y
+  | And _ x y
+  | Or _ x y => [x; y]
+  | Not _ x | Id _ x | Br x _ _ | Ret (Some x) => [x]
+  | Call _ _ args | Print args => args
+  | Jmp _ | Const _ _ | Nop | Ret None => []
+  end.
+
+(** Extract the names of functions referenced by an instruction *)
+Definition funcs (instr : Instruction.t) : list function :=
+  if instr is Call _ func _ then [func] else [].
+
+(** Extract the names of labels referenced by an instruction *)
+Definition labels (instr : Instruction.t) : list label :=
+  match instr with
+  | Jmp l => [l]
+  | Br _ t f => [t; f]
+  | _ => []
+  end.
+
+(** If [value] an instruction [const lit], return [inr lit].
+    Otherwise, return an error. *)
+Definition value (instr : Instruction.t) : option Literal.t :=
+  if instr is Const _ lit then Some lit else None.
+
+(** Attempt to decode exactly two operands in list format from
+    a JSON *)
+Definition decode_op_pair j : string + (operand * operand) :=
+  @decode (operand * operand) decode_pair j.
+
+Import MonadLetNotation.
+
+(** [decode_binary op j] is [inr (op dst x y)] where 
+    [dst] is the destination decoded from [j], and [x], [y]
+    are the two operands decoded from [j]. If [j] is malformed, 
+    return an error. *)
+Definition decode_binary (op : Dest.t -> operand -> operand -> t) j : string + t :=
+  let* dest := decode j in
+  let* (x, y) := decode_op_pair =<< member "args" j in
+  ret (op dest x y).
+
+(** Decode the element of a singleton json array *)
+Definition decode_singleton {T} `{JDecode T} j : string + T :=
+  lst <- @decode (list T) decode__list j ;;
+  match lst with
+  | [h] => ret h
+  | _ => inl "Expected singleton array"
+  end.
+
+(** [decode_unary op j] is [inr (op dst x)] where 
+    [dst] is the destination decoded from [j], and [x]
+    is the single operand decoded from [j] *)
+Definition decode_unary (op : Dest.t -> operand -> t) j : string + t :=
+  let* dest := decode j in
+  let* arg := decode_singleton =<< member "args" j in
+  ret (op dest arg).
+
+(** Decode a [const] instruction *)
+Definition decode_const j : string + t :=
+  let* dest := decode j in
+  let* lit := decode =<< member "value" j in
+  ret (Const dest lit).
+
+(** Decode a [call] instruction *)
+Definition decode_call j : string + t :=
+  let* func := decode_singleton =<< member "funcs" j in
+  let* args := @decode (list operand) decode__list =<< member "args" j in
+  match decode j with
+  | inr dest => ret (Call (Some dest) func args)
+  | inl _ => ret (Call None func args)
+  end.
+
+(** Decode a [jmp] instruction *)
+Definition decode_jmp j : string + t :=
+  Jmp <$> (decode_singleton =<< member "labels" j).
+
+(** Decode a [br] instruction *)
+Definition decode_br j :=
+  let* cond := decode_singleton =<< member "args" j in
+  let* labels := member "labels" j in
+  let* (t, f) := @decode (label * label) decode_pair labels in
+  ret (Br cond t f).
+
+(** Decode a [rets] instruction *)
+Definition decode_ret j : string + t :=
+  let* args := @decode (list operand) decode__list =<< member "args" j in
+  match args with
+  | [value] => ret (Ret (Some value))
+  | [] => ret (Ret None)
+  | _ => inl "Too many arguments to return"
+  end.
+
+(** Decode a [print] instruction *)
+Definition decode_print j :=
+  let* args := @decode (list operand) decode__list =<< member "args" j in
+  ret (Print args).
+
+Global Instance JDecode_Typ : JDecode t :=
+  fun j =>
+    op <- (get_string =<< member "op" j) ;;
+    match op with
+    | "add" => decode_binary Add j
+    | "mul" => decode_binary Mul j
+    | "sub" => decode_binary Sub j
+    | "div" => decode_binary Div j
+    | "eq" => decode_binary Eq j
+    | "lt" => decode_binary Lt j
+    | "gt" => decode_binary Gt j
+    | "le" => decode_binary Le j
+    | "ge" => decode_binary Ge j
+    | "not" => decode_unary Not j
+    | "and" => decode_binary And j
+    | "or" => decode_binary Or j
+    | "jmp" => decode_jmp j
+    | "br" => decode_br j
+    | "call" => decode_call j
+    | "ret" => decode_ret j
+    | "const" => decode_const j
+    | "id" => decode_unary Id j
+    | "print" => decode_print j
+    | "nop" => ret Nop
+    | _ => inl "Invalid opcode"
+    end.
+
