bril-coq/theories/Argument.v
@@ -1,5 +1,8 @@
 Require Import Coq.Strings.String.
+From ExtLib Require Import Monad.
+From JSON Require Import JSON Decode Encode.
 
+Require Import Util.JSON.
 Require Typ.
 
 (** Represents an argument to a Bril function *)
@@ -9,3 +12,17 @@ Record t := {
   (** The Bril type of the argument*)
   typ : Typ.t;
 }.
+
+Global Instance JDecode_Argument : JDecode t :=
+  fun j =>
+    name <- (get_string =<< member "name" j) ;;
+    typ <- (decode =<< member "type" j) ;;
+    ret {| name := name; typ := typ |}.
+
+Global Instance JEncode_Argument : JEncode t :=
+  fun arg =>
+    JSON__Object
+      [
+        ("name", encode arg.(name));
+        ("type", encode arg.(typ))
+      ].
