bril-coq/theories/Literal.v
@@ -1,4 +1,6 @@
 Require Import Coq.Numbers.BinNums.
+From ExtLib Require Import Monad.
+From JSON Require Import JSON Decode Encode.
 
 (** Represents a literal Bril constant *)
 Variant t :=
@@ -6,3 +8,20 @@ Variant t :=
   | Int (i : Z)
   (** A literal boolean *)
   | Bool (b : bool).
+
+Global Instance JDecode_Literal : JDecode t :=
+  fun j =>
+    match j with
+    | JSON__Number i => ret (Int i)
+    | JSON__True => ret (Bool true)
+    | JSON__False => ret (Bool false)
+    | _ => inl "Cannot decode JSON"
+    end.
+
+Global Instance JEncode_Literal : JEncode t :=
+  fun typ =>
+    match typ with
+    | Int i => JSON__Number i
+    | Bool true => JSON__True
+    | Bool false => JSON__False
+    end.
