bril-coq/theories/Program.v
@@ -1,3 +1,4 @@
-Require Import Bril.Function.
+Require Function.
 
+ (** A Bril program is represented by a list of functions *)
 Definition t := list Function.t.
