bril-coq/theories/Typ.v
@@ -1,3 +1,21 @@
+From ExtLib Require Import Monad.
+From JSON Require Import JSON Decode Encode.
+Require Import Util.JSON.
 
 (** Represents the type of a Bril value *)
 Variant t := Int | Bool.
+
+Global Instance JDecode_Typ : JDecode t :=
+  fun j =>
+    match j with
+    | JSON__String "int" => ret Int
+    | JSON__String "bool" => ret Bool
+    | _ => inl "Cannot decode JSON"
+    end.
+
+Global Instance JEncode_Typ : JEncode t :=
+  fun typ =>
+    match typ with
+    | Int => JSON__String "int"
+    | Bool => JSON__String "bool"
+    end.
