bril-coq/theories/Util/JSON.v
@@ -1,0 +1,21 @@
+From Coq Require Import Lists.List Strings.String.
+From ExtLib Require Import EitherMonad.
+From JSON Require Import JSON.
+
+Import IfNotations.
+
+Open Scope string_scope.
+
+(** [member key j] is the value associated with key [key] of [json] *)
+Definition member (key : string) (j : json) : string + json :=
+  if j is JSON__Object entries then
+    match List.find (fun '(key', _) => key =? key') entries with
+    | Some (_, value) => ret value
+    | None => inl ("JSON object does not have property " ++ key)
+    end
+  else
+    inl "Cannot extract member from non-object".
+
+(** [get_string j] is the string wrapped by json [j] *)
+Definition get_string (j : json) : string + string :=
+  if j is JSON__String s then ret s else inl "Expected string".
